\documentclass[tf-tutorial-all.tex]{subfiles}
\begin{document}

\begin{truefalse}
Let $X \sim \Pois{\lambda}$ then $$\left( \frac{ \sum^{n}_{i=1} X_{i}}{\sqrt{n} \sqrt{\lambda}} - \sqrt{n}\sqrt{\lambda} \right) \to \Norm{0,1} \quad \text{as } n \to \infty$$.
\begin{solution}
Correct\\
$$\sqrt{n} \left( \frac{ \bar{X}_{n}  - \lambda}{\sqrt{\lambda}}  \right) $$ 
$$\sqrt{n} \left( \frac{ \frac{1}{n} \sum^{n}_{i=1} X_{i}  }{\sqrt{\lambda}} - \sqrt{\lambda}  \right) $$ 
$$ = \left( \frac{ \sum^{n}_{i=1} X_{i}}{\sqrt{n}\lambda} - \sqrt{n}\sqrt{\lambda} \right)$$
$$
\to \Norm{0,1} \quad \text{as } n \to \infty$$
More generally
$$ \sqrt{n}\left(\frac{\bar{X}_{n} - \mu}{\sigma}  \right) \to \Norm{0,1} \quad \text{as } n \to \infty$$.
\end{solution}
\end{truefalse}

\end{document}
